Update Q4.dfy

LAB3/Q4.dfy
@@ -1,12 +1,21 @@
 method ComputeFact(n : nat) returns (res : nat)
-requires n > 0;
-ensures res == fact(n);
+  requires n > 0;
+  ensures res == fact(n);
+ {
+  res := 1;
+  var i := 2;
+  while (i <= n)
+  invariant i <= n + 1;
+  invariant res == fact(i-1);
+  {
+    res := res * i;
+    i := i + 1;
+  }
+ }
+
+ function fact(m: int): int
+  requires 0 <= m;
+  ensures 1 <= fact(m);
 {
-res := 1;
-var i := 2;
-while (i <= n)
-{
-res := res * i;
-i := i + 1;
-}
-}
+ if m == 0 then 1 else fact(m-1) * m
+ } 
